Enhance the lre rules
Combines the big-step and small-step version of lre. User can choose either small-step or big-step when verify a specific event

Ann_PiCore_RG_IFS.thy
@@ -813,30 +813,26 @@ lemma reachable_impl_cpts: "reachable C1 C2 \<Longrightarrow> \<exists>c. c\<in>
 lemma reachable0_impl_cpts: "reachable0 C \<Longrightarrow> \<exists>c. c\<in>cpts_pes \<and> c!0 = C0 \<and> last c = C"
   using reachable_impl_cpts reachable0_def by simp
 
+
 definition locally_respect_events :: "bool" where
-  "locally_respect_events \<equiv> \<forall>ef. ef\<in>all_evts pesf  \<longrightarrow> \<turnstile>\<^sub>l\<^sub>r the (body_e (E\<^sub>e ef)) sat\<^sub>p (E\<^sub>e ef)"
-
-definition locally_respect_events_guar :: "bool" where
-  "locally_respect_events_guar \<equiv> \<forall>ef u s1 s2 . ef\<in>all_evts pesf \<and> (s1,s2) \<in> Guar\<^sub>e ef \<longrightarrow> 
-                                    ((dome s1 (E\<^sub>e ef)) \<setminus>\<leadsto> u \<longrightarrow> s1 \<sim>u\<sim> s2)"
-
+  "locally_respect_events \<equiv> \<forall>ef. ef\<in>all_evts pesf \<longrightarrow> ( (\<turnstile>\<^sub>l\<^sub>r the (body_e (E\<^sub>e ef)) sat\<^sub>p (E\<^sub>e ef)) \<or>
+   (\<forall>u s1 s2. (s1, s2) \<in> Guar\<^sub>e ef \<longrightarrow> ((dome s1 (E\<^sub>e ef)) \<setminus>\<leadsto> u \<longrightarrow> s1 \<sim>u\<sim> s2)))"
 
 definition step_consistent_events :: "bool" where
   "step_consistent_events \<equiv> \<forall>ef. ef\<in>all_evts pesf  \<longrightarrow> \<turnstile>\<^sub>s\<^sub>c the (body_e (E\<^sub>e ef)) sat\<^sub>p (E\<^sub>e ef)"
 
-
-
 lemma rg_lr_imp_lr: "locally_respect_events \<Longrightarrow> locally_respect"
 proof-
   assume p0: "locally_respect_events"
-  then have p1: "\<forall>ef. ef\<in>all_evts pesf  \<longrightarrow> (\<exists>\<S>. (E\<^sub>e ef) \<in> \<S> \<and> locally_respect_e \<S> (E\<^sub>e ef))"
+  then have p1: "\<forall>ef. ef\<in>all_evts pesf  \<longrightarrow> ((\<exists>\<S>. (E\<^sub>e ef) \<in> \<S> \<and> locally_respect_e \<S> (E\<^sub>e ef)) \<or> 
+                 (\<forall>u s1 s2. (s1, s2) \<in> Guar\<^sub>e ef \<longrightarrow> ((dome s1 (E\<^sub>e ef)) \<setminus>\<leadsto> u \<longrightarrow> s1 \<sim>u\<sim> s2)))"
     using all_evts_are_basic locally_respect_events_def lr_e_Basic1 by blast
   show ?thesis
   proof-
     {
       fix a u C
       assume a0: "reachable0 C"
-        and  a1: "(domain (a::('l,'k,'s,'d) action)) \<setminus>\<leadsto> u"
+         and a1: "(domain (a::('l,'k,'s,'d) action)) \<setminus>\<leadsto> u"
       have "\<forall> C'. (C'\<in>nextc C a) \<longrightarrow> (C \<sim>.u.\<sim> C')"
       proof-
         {
@@ -846,64 +842,65 @@ proof-
           then have b2: "(C -pes-(actk a)\<rightarrow> C') \<and> ((\<exists>e k. actk a = ((EvtEnt e)\<sharp>k) \<and> eventof a = e 
                           \<and> dome (gets C) e = domain a) \<or> (\<exists>c k. actk a = ((Cmd c)\<sharp>k) \<and> 
                           eventof a = (getx C) k \<and> dome (gets C) (eventof a) = domain a))"
-              by (simp add:step_def)
-            obtain act_k and e and d where b3: "a = \<lparr>actk = act_k,eventof = e, domain=d\<rparr>"
-              using action.cases by blast 
-            with b2 have b4: "(C -pes-act_k\<rightarrow> C') \<and> ((\<exists>e k. act_k = ((EvtEnt e)\<sharp>k) \<and> eventof a = e 
-                              \<and> dome (gets C) e = domain a) \<or> (\<exists>c k. act_k = ((Cmd c)\<sharp>k) \<and> 
-                              eventof a = (getx C) k \<and> dome (gets C) (eventof a) = domain a))"
-              by simp
-            obtain act and k where b5: "act_k = act\<sharp>k"
-              by (metis actk.cases get_actk_def)
-            obtain pes1 and s1 and x1 where b6: "C = (pes1,s1,x1)" using prod_cases3 by blast 
-            obtain pes2 and s2 and x2 where b7: "C' = (pes2,s2,x2)" using prod_cases3 by blast
-            from b4 b5 b6 b7 have "\<exists>es'. ((pes1 k, s1, x1) -es-(act\<sharp>k)\<rightarrow> (es', s2, x2)) \<and> pes2 = pes1(k:=es')"
-              using pestran_estran by force
-            then obtain es' where b8: "((pes1 k, s1, x1) -es-(act\<sharp>k)\<rightarrow> (es', s2, x2)) \<and> pes2 = pes1(k:=es')" by auto
-            from b5 have "C \<sim>.u.\<sim> C'"
-            proof(induct act)
-              case (Cmd x)
-              assume c0: "act_k = Cmd x\<sharp>k"
-              from a0 have "\<exists>as. (C0,C) \<in> run as" by (simp add:reachable0_def reachable_def)
-              then obtain as where "(C0,C) \<in> run as" by auto
-              then have "(\<exists>c. c\<in>cpts_pes \<and> c!0 = C0 \<and> last c = C \<and> Suc (length as) = length c \<and>
-                              (\<forall>j. Suc j < length c \<longrightarrow> (c!j-pes-(actk (as!j))\<rightarrow>c!Suc j)) )"
-                using run_is_cpt by blast
-              then obtain c where c1: "c\<in>cpts_pes \<and> c!0 = C0 \<and> last c = C \<and> Suc (length as) = length c \<and>
-                              (\<forall>j. Suc j < length c \<longrightarrow> (c!j-pes-(actk (as!j))\<rightarrow>c!Suc j))" by auto
-              with b1 have c2: "c@[C']\<in>cpts_pes" using cpts_pes_onemore step_def
-                by (metis (no_types, lifting) b4 cpts_pes_not_empty last_conv_nth)
-              with c1 have c3: "c @ [C'] \<in> cpts_of_pes (paresys_spec pesf) s0 x0" 
-                using cpts_of_pes_def[of "paresys_spec pesf" s0 x0] C0_ParSys
-                by (smt cpts_pes_not_empty length_greater_0_conv mem_Collect_eq nth_append)
-              moreover
-              from c1 have c4: "(c @ [C']) ! (length (c @ [C']) - 2) = C"
-                by (metis Suc_1 diff_Suc_1 diff_Suc_Suc last_conv_nth length_0_conv length_append_singleton
-                    lessI nat.simps(3) nth_append)
-              moreover
-              have c5: "(c @ [C']) ! (length (c @ [C']) - 1) = C'" by simp
-              moreover
-              from b1 c1 have c50: "\<forall>j. Suc j < length (c @ [C']) \<longrightarrow> 
-                   ((c @ [C'])!j-pes-(actk ((as@[a])!j))\<rightarrow>(c @ [C'])!Suc j)"
-                by (smt Suc_1 Suc_lessI Suc_less_eq action.simps(1) b3 b4 c4 diff_Suc_1 diff_Suc_Suc 
-                    length_append_singleton nth_append nth_append_length) 
-
-            from c3 c50 have c51: "\<forall>k i. Suc i < length (c @ [C']) \<longrightarrow>
-                      (\<exists>ca. (c @ [C']) ! i -pes-Cmd ca\<sharp>k\<rightarrow> (c @ [C']) ! Suc i) \<longrightarrow>
-                      (\<exists>ef\<in>all_evts pesf. getx ((c @ [C']) ! i) k = fst ef) " 
-              using all_evts_are_basic cur_evt_in_specevts [of "c@[C']" pesf] by (metis E\<^sub>e_def)
+            by (simp add:step_def)
+          obtain act_k and e and d where b3: "a = \<lparr>actk = act_k,eventof = e, domain=d\<rparr>"
+            using action.cases by blast
+          with b2 have b4: "(C -pes-act_k\<rightarrow> C') \<and> ((\<exists>e k. act_k = ((EvtEnt e)\<sharp>k) \<and> eventof a = e 
+                             \<and> dome (gets C) e = domain a) \<or> (\<exists>c k. act_k = ((Cmd c)\<sharp>k) \<and> 
+                             eventof a = (getx C) k \<and> dome (gets C) (eventof a) = domain a))"
+            by simp
+          obtain act and k where b5: "act_k = act\<sharp>k"
+            by (metis actk.cases get_actk_def)
+          obtain pes1 and s1 and x1 where b6: "C = (pes1,s1,x1)" using prod_cases3 by blast 
+          obtain pes2 and s2 and x2 where b7: "C' = (pes2,s2,x2)" using prod_cases3 by blast
+          from b4 b5 b6 b7 have "\<exists>es'. ((pes1 k, s1, x1) -es-(act\<sharp>k)\<rightarrow> (es', s2, x2)) \<and> pes2 = pes1(k:=es')"
+            using pestran_estran by force
+          then obtain es' where b8: "((pes1 k, s1, x1) -es-(act\<sharp>k)\<rightarrow> (es', s2, x2)) \<and> pes2 = pes1(k:=es')" by auto
+          from b5 have "C \<sim>.u.\<sim> C'"
+          proof(induct act)
+            case (Cmd x) 
+            assume c0: "act_k = Cmd x\<sharp>k"
+            from a0 have "\<exists>as. (C0,C) \<in> run as" by (simp add:reachable0_def reachable_def)
+            then obtain as where "(C0,C) \<in> run as" by auto
+            then have "(\<exists>c. c\<in>cpts_pes \<and> c!0 = C0 \<and> last c = C \<and> Suc (length as) = length c \<and>
+                       (\<forall>j. Suc j < length c \<longrightarrow> (c!j-pes-(actk (as!j))\<rightarrow>c!Suc j)) )"
+              using run_is_cpt by blast
+            then obtain c where c1: "c\<in>cpts_pes \<and> c!0 = C0 \<and> last c = C \<and> Suc (length as) = length c \<and>
+                        (\<forall>j. Suc j < length c \<longrightarrow> (c!j-pes-(actk (as!j))\<rightarrow>c!Suc j))" by auto
+            with b1 have c2: "c@[C']\<in>cpts_pes" using cpts_pes_onemore step_def
+              by (metis (no_types, lifting) b4 cpts_pes_not_empty last_conv_nth)
+            with c1 have c3: "c @ [C'] \<in> cpts_of_pes (paresys_spec pesf) s0 x0" 
+              using cpts_of_pes_def[of "paresys_spec pesf" s0 x0] C0_ParSys
+              by (smt cpts_pes_not_empty length_greater_0_conv mem_Collect_eq nth_append)
+            moreover
+            from c1 have c4: "(c @ [C']) ! (length (c @ [C']) - 2) = C"
+              by (metis Suc_1 diff_Suc_1 diff_Suc_Suc last_conv_nth length_0_conv length_append_singleton
+                  lessI nat.simps(3) nth_append)
+            moreover
+            have c5: "(c @ [C']) ! (length (c @ [C']) - 1) = C'" by simp
+            moreover
+            from b1 c1 have c50: "\<forall>j. Suc j < length (c @ [C']) \<longrightarrow> ((c @ [C'])!j-pes-(actk ((as@[a])!j))
+                    \<rightarrow>(c @ [C'])!Suc j)"
+              by (smt Suc_1 Suc_lessI Suc_less_eq action.simps(1) b3 b4 c4 diff_Suc_1 diff_Suc_Suc
+                  length_append_singleton nth_append nth_append_length) 
+            ultimately have r1: "(gets C, gets C')\<in>Guar\<^sub>f (the (evtrgfs (getx C k)))" 
+              using b1 b3 b4 c0 c1 act_cptpes_sat_guar_curevt_new2 [rule_format, of pesf "{s0}" UNIV s0 evtrgfs "c@[C']"]
+                     step_def[of a] parsys_sat_rg all_evts_are_basic evt_in_parsys_in_evtrgfs
+              by (smt One_nat_def Suc_1 append_is_Nil_conv butlast_snoc diff_Suc_1  diff_Suc_eq_diff_pred 
+                 diff_Suc_less insertI1 length_butlast length_greater_0_conv not_Cons_self2)      
+            from c3 c50 have c51: "\<forall>k i. Suc i < length (c @ [C']) \<longrightarrow> (\<exists>ca. (c @ [C']) ! i -pes-Cmd ca\<sharp>k\<rightarrow> 
+                    (c @ [C']) ! Suc i) \<longrightarrow> (\<exists>ef\<in>all_evts pesf. getx ((c @ [C']) ! i) k = fst ef) " 
+              using all_evts_are_basic cur_evt_in_specevts [of "c@[C']" pesf] by (metis E\<^sub>e_def) 
             moreover
             from b1 b3 c0 have c52: "C-pes-Cmd x\<sharp>k\<rightarrow>C'" using step_def by simp
-
-
             ultimately have "(\<exists>ef\<in>all_evts pesf. getx C k = fst ef)"
               using c1 c4 c5
-            proof-
+            proof -
               have f1: "\<forall>k n. \<not> Suc n < length (c @ [C']) \<or>
-                         (\<forall>ca. ((c @ [C']) ! n, Cmd ca\<sharp>k, (c @ [C']) ! Suc n) \<notin> pestran) \<or> 
+                        (\<forall>ca. ((c @ [C']) ! n, Cmd ca\<sharp>k, (c @ [C']) ! Suc n) \<notin> pestran) \<or> 
                         (\<exists>p. p \<in> all_evts pesf \<and> fst p = getx ((c @ [C']) ! n) k)"
                 by (metis c51)
-              from c1 have f2: "\<forall>ps. c ! length as = (c @ ps) ! length as" 
+              have f2: "\<forall>ps. c ! length as = (c @ ps) ! length as"
                 by (metis (no_types) c1 lessI nth_append)
               have "c ! length as = C"
                 by (metis (no_types) append_Nil c1 diff_Suc_1 id_take_nth_drop last_length 
@@ -911,55 +908,62 @@ proof-
               then show ?thesis
                 using f2 f1 by (metis c52 c1 c5 diff_Suc_1 length_append_singleton lessI)
             qed
-
-            then obtain ef where c12: "ef\<in>all_evts pesf \<and> getx C k = E\<^sub>e ef"
-              by (metis E\<^sub>e_def)
-            from c0 have c12_1: "\<not>(\<exists>e k. act_k = EvtEnt e\<sharp>k)"
+            then obtain ef where c7: "ef\<in>all_evts pesf \<and> getx C k = fst ef" by auto
+            from c0 have "\<not>(\<exists>e k. act_k = EvtEnt e\<sharp>k)"
               by (simp add: get_actk_def) 
-            with b3 b4 c0 have c13: "\<exists>x. act_k = Cmd x\<sharp>k \<and> eventof a = getx C k \<and> dome (gets C) (eventof a) = domain a"
+            with b3 b4 c0 have c70: "\<exists>x k. act_k = Cmd x\<sharp>k \<and> eventof a = getx C k \<and> dome (gets C) (eventof a) = domain a"
+              by simp
+            with a1 b3 c0 have c8: "eventof a = getx C k \<and> dome (gets C) (eventof a) = domain a" 
               by (metis actk.iffs get_actk_def)
-            with a1 b3 c0 have c14: "eventof a = getx C k \<and> dome (gets C) (eventof a) = domain a"
-              by force
 
-            let ?pes = "paresys_spec pesf"
-            let ?i = "length (c @ [C']) - 2"
-            have "\<exists>\<S>. AnonyEvent x \<in> \<S> \<and> locally_respect_e \<S> (E\<^sub>e ef)"
-            proof-
-              {
-                have "\<exists>el j.  getspc_e (el!0) = getx C k \<and> j < length el \<and> 
-                     el!j = rm_evtsys1 ((getspc C k), gets C, getx C) \<and> el \<in> cpts_ev \<and> el \<in> preserves_e"
-                  using act_cptpes_sat_e_sim[rule_format, of pesf "{s0}" UNIV s0 evtrgfs "c @ [C']"
+            with a1 b3 b6 c7 have c9 : "(dome s1  (E\<^sub>e ef)) \<setminus>\<leadsto> u" 
+              using gets_def E\<^sub>e_def by (metis fst_conv snd_conv)
+
+            from p1 c7 have c10: "(\<exists>\<S>. (E\<^sub>e ef) \<in> \<S> \<and> locally_respect_e \<S> (E\<^sub>e ef)) \<or> 
+            (\<forall>u s1 s2. (s1, s2) \<in> Guar\<^sub>e ef \<longrightarrow> ((dome s1 (E\<^sub>e ef)) \<setminus>\<leadsto> u \<longrightarrow> s1 \<sim>u\<sim> s2))"
+              by presburger
+            then have " s1 \<sim>u\<sim> s2"
+            proof
+              assume d0: "\<exists>\<S>. E\<^sub>e ef \<in> \<S> \<and> locally_respect_e \<S> (E\<^sub>e ef)"
+              let ?pes = "paresys_spec pesf"
+              let ?i = "length (c @ [C']) - 2"
+              have "\<exists>\<S>. AnonyEvent x \<in> \<S> \<and> locally_respect_e \<S> (E\<^sub>e ef)"
+              proof-
+                {
+                  have "\<exists>el j.  getspc_e (el!0) = getx C k \<and> j < length el \<and>  el!j = rm_evtsys1 
+                        ((getspc C k), gets C, getx C) \<and> el \<in> cpts_ev \<and> el \<in> preserves_e"
+                    using act_cptpes_sat_e_sim[rule_format, of pesf "{s0}" UNIV s0 evtrgfs "c @ [C']"
                         x0 ?i k] parsys_sat_rg all_evts_are_basic evt_in_parsys_in_evtrgfs c1 c3 c4 c5 c50 c52
-                  by (smt One_nat_def Suc_1 Suc_diff_Suc Suc_less_eq diff_less insertI1 
-                      length_append_singleton zero_less_Suc)
-                then obtain el and j where e0: "getspc_e (el!0) = getx C k \<and> j < length el \<and> 
+                    by (smt One_nat_def Suc_1 Suc_diff_Suc Suc_less_eq diff_less insertI1
+                        length_append_singleton zero_less_Suc)
+                  then obtain el and j where e0: "getspc_e (el!0) = getx C k \<and> j < length el \<and> 
                      el!j = rm_evtsys1 ((getspc C k), gets C, getx C) \<and> el \<in> cpts_ev \<and> el \<in> preserves_e"
-                  by auto
-                with c12 have c120: "getspc_e (el!0) = E\<^sub>e ef \<and> j < length el \<and> 
+                    by auto
+                with c7 have e1: "getspc_e (el!0) = E\<^sub>e ef \<and> j < length el \<and> 
                                el!j = rm_evtsys1 ((getspc C k), gets C, getx C) 
-                               \<and> el \<in> cpts_ev \<and> el \<in> preserves_e" by simp
-                with c12 p1 have "\<exists>\<S>. (E\<^sub>e ef) \<in> \<S> \<and> locally_respect_e \<S> (E\<^sub>e ef)" by blast
-                then obtain \<S> where e1: "(E\<^sub>e ef) \<in> \<S> \<and> locally_respect_e \<S> (E\<^sub>e ef)" by auto
+                               \<and> el \<in> cpts_ev \<and> el \<in> preserves_e"  by (simp add: E\<^sub>e_def)
+                with c7 d0 have "\<exists>\<S>. (E\<^sub>e ef) \<in> \<S> \<and> locally_respect_e \<S> (E\<^sub>e ef)" by blast
+                then obtain \<S> where e2: "(E\<^sub>e ef) \<in> \<S> \<and> locally_respect_e \<S> (E\<^sub>e ef)" by auto
 
                 from b5 b8 b4 c0 have "\<exists>es. getspc C k = EvtSeq (AnonyEvent x) es"
                   by (metis  pes_cmd_tran_anonyevt pesconf_trip)
                 then obtain es where "getspc C k = EvtSeq (AnonyEvent x) es" by auto
-                with e0 b8 have e2: "el!j = (AnonyEvent x, s1, x1)" 
+                with e0 b8 have e3: "el!j = (AnonyEvent x, s1, x1)" 
                   using rm_evtsys1_def 
                   by (metis EvtSeqrm Pair_inject b6 esconf_trip pesconf_trip)
-                with e0 e1 e2 c120 have "AnonyEvent x \<in> \<S>"
+                with e0 e1 e2 e3 have "AnonyEvent x \<in> \<S>"
                   using locally_respect_forall[of "E\<^sub>e ef" \<S> "E\<^sub>e ef" el j]
                   by (metis getspc_e_def fstI)
-                with e1 show ?thesis by auto
+                with e2 show ?thesis by auto
               }
             qed
 
-            then obtain \<S> where d0: "AnonyEvent x \<in> \<S> \<and> locally_respect_e \<S> (E\<^sub>e ef)" by auto
+            then obtain \<S> where d1: "AnonyEvent x \<in> \<S> \<and> locally_respect_e \<S> (E\<^sub>e ef)" by auto
 
-            have d1: "ann_preserves_e (AnonyEvent x) s1"
+            have d2: "ann_preserves_e (AnonyEvent x) s1"
             proof- 
               {
-                from c3 c50 have "c @ [C'] \<in> preserves_pes" 
+                from c3 c50 have "c @ [C'] \<in> preserves_pes"
                   using run_cpt_preserves pes_tran_not_etran1 by blast
                 with c4 b6 have "ann_preserves_pes pes1 s1"
                   apply (simp add: preserves_pes_def)
@@ -967,159 +971,41 @@ proof-
                   by (simp add: getspc_def gets_def)
                 then have f0 : "ann_preserves_es (pes1 k) s1"
                   by (simp add: ann_preserves_pes_def)
-            from b5 b8 c52 c0 have "\<exists>es. pes1 k = EvtSeq (AnonyEvent x) es"
-              by (metis  evtseq_cmd_tran_anonyevt)
-            then obtain es where "pes1 k = EvtSeq (AnonyEvent x) es" by auto
-            with f0 have "ann_preserves_e (AnonyEvent x) s1"
-              by (simp add: ann_preserves_es_def)
-          }
-          then show ?thesis by auto
+                from b5 b8 c52 c0 have "\<exists>es. pes1 k = EvtSeq (AnonyEvent x) es"
+                  by (metis  evtseq_cmd_tran_anonyevt)
+                then obtain es where "pes1 k = EvtSeq (AnonyEvent x) es" by auto
+                with f0 have "ann_preserves_e (AnonyEvent x) s1"
+                  by (simp add: ann_preserves_es_def)
+              }
+              then show ?thesis by auto
+            qed
+
+            with b6 b7 c52 c9 d1 show ?thesis 
+              by (metis locally_next_state pes_cmd_tran_anonyevt1)
+          next
+            assume f0: "\<forall>u s1 s2. (s1, s2) \<in> Guar\<^sub>e ef \<longrightarrow> dome s1 (E\<^sub>e ef) \<setminus>\<leadsto> u \<longrightarrow> s1 \<sim>u\<sim> s2"
+            from p1 b6 b7 c7 c8 r1 have "(gets C, gets C')\<in>Guar\<^sub>e ef"
+              using evt_in_parsys_in_evtrgfs Guar\<^sub>f_def E\<^sub>e_def Guar\<^sub>e_def by metis
+            with f0 show ?thesis using p1 b6 b7 c7 c8 a1 vpeqc_def E\<^sub>e_def
+              by (metis fst_conv gets_def snd_conv)
+          qed
+
+          then show ?case
+            by (simp add: b6 b7 gets_def vpeqc_def)
+        next
+          case (EvtEnt x)
+          from b5 b8 have "s1 = s2" 
+            using entevt_notchgstate by (metis EvtEnt.prems evtent_is_basicevt)
+          with b6 b7 show ?case by (simp add: gets_def vpeqc_def vpeq_reflexive)
         qed
-
-        from b6 b7 c52 have "\<exists>e2. (AnonyEvent x, s1, x1) -et-Cmd x\<sharp>k\<rightarrow> (e2, s2, x2)"
-          by (meson pes_cmd_tran_anonyevt1)
-        then obtain e2 where d2 : "(AnonyEvent x, s1, x1) -et-Cmd x\<sharp>k\<rightarrow> (e2, s2, x2)"
-          by auto
-        from a1 b6 c12 c14 have d3: "(dome s1 (E\<^sub>e ef)) \<setminus>\<leadsto> u"
-          by (metis  fst_conv gets_def prod.sel(2))
-
-        with d0 d1 d2 d3 have "s1 \<sim>u\<sim> s2"
-          by (simp add: locally_next_state)
-
-        with b6 b7 show ?case by (simp add: gets_def vpeqc_def)
-
-      next
-        case (EvtEnt x) 
-        from b5 b8 have "s1 = s2" 
-          using entevt_notchgstate by (metis EvtEnt.prems evtent_is_basicevt)
-        with b6 b7 show ?case by (simp add: gets_def vpeqc_def vpeq_reflexive)
-      qed
-    }
-    then show ?thesis by auto
-  qed
-}
+      }
+      then show ?thesis by auto
+    qed
+  }
   then show ?thesis using locally_respect_def by simp
 qed
 qed
 
-lemma rg_lr_guar_imp_lr: "locally_respect_events_guar \<Longrightarrow> locally_respect"
-  proof -
-    assume p0: "locally_respect_events_guar"
-    then have p1: " \<forall>ef u s1 s2. ef\<in>all_evts pesf \<and> (s1,s2) \<in> Guar\<^sub>e ef \<longrightarrow> 
-                                    ((dome s1 (E\<^sub>e ef)) \<setminus>\<leadsto> u \<longrightarrow> s1 \<sim>u\<sim> s2)"
-      by (simp add:locally_respect_events_guar_def)
-    show ?thesis
-      proof -
-      {
-        fix a u C
-        assume a0: "reachable0 C"
-          and  a1: "(domain (a::('l,'k,'s,'d) action)) \<setminus>\<leadsto> u"
-        have "\<forall> C'. (C'\<in>nextc C a) \<longrightarrow> (C \<sim>.u.\<sim> C')"
-          proof -
-          {
-            fix C'
-            assume b0: "C'\<in>nextc C a"
-            then have b1: "(C,C')\<in>step a" by (simp add:nextc_def)
-            then have b2: "(C -pes-(actk a)\<rightarrow> C') \<and>
-                            ((\<exists>e k. actk a = ((EvtEnt e)\<sharp>k) \<and> eventof a = e \<and> dome (gets C) e = domain a) \<or>
-                             (\<exists>c k. actk a = ((Cmd c)\<sharp>k) \<and> eventof a = (getx C) k \<and> dome (gets C) (eventof a) = domain a))"
-              by (simp add:step_def)
-            obtain act_k and e and d where b3: "a = \<lparr>actk = act_k,eventof = e, domain=d\<rparr>"
-              using action.cases by blast 
-            with b2 have b4: "(C -pes-act_k\<rightarrow> C') \<and> 
-                              ((\<exists>e k. act_k = ((EvtEnt e)\<sharp>k) \<and> eventof a = e \<and> dome (gets C) e = domain a) \<or>
-                             (\<exists>c k. act_k = ((Cmd c)\<sharp>k) \<and> eventof a = (getx C) k \<and> dome (gets C) (eventof a) = domain a))"
-              by simp
-            obtain act and k where b5: "act_k = act\<sharp>k"
-              by (metis actk.cases get_actk_def) 
-            obtain pes1 and s1 and x1 where b6: "C = (pes1,s1,x1)" using prod_cases3 by blast 
-            obtain pes2 and s2 and x2 where b7: "C' = (pes2,s2,x2)" using prod_cases3 by blast
-            from b4 b5 b6 b7 have "\<exists>es'. ((pes1 k, s1, x1) -es-(act\<sharp>k)\<rightarrow> (es', s2, x2)) \<and> pes2 = pes1(k:=es')" 
-              using pestran_estran by force
-            then obtain es' where b8: "((pes1 k, s1, x1) -es-(act\<sharp>k)\<rightarrow> (es', s2, x2)) \<and> pes2 = pes1(k:=es')" by auto
-
-            from b5 have "C \<sim>.u.\<sim> C'"
-              proof(induct act)
-                case (Cmd x) 
-                assume c0: "act_k = Cmd x\<sharp>k"
-                from a0 have "\<exists>as. (C0,C) \<in> run as" by (simp add:reachable0_def reachable_def)
-                then obtain as where "(C0,C) \<in> run as" by auto
-                then have "(\<exists>c. c\<in>cpts_pes \<and> c!0 = C0 \<and> last c = C \<and> Suc (length as) = length c \<and>
-                              (\<forall>j. Suc j < length c \<longrightarrow> (c!j-pes-(actk (as!j))\<rightarrow>c!Suc j)) )"
-                  using run_is_cpt by blast
-                then obtain c where c1: "c\<in>cpts_pes \<and> c!0 = C0 \<and> last c = C \<and> Suc (length as) = length c \<and>
-                              (\<forall>j. Suc j < length c \<longrightarrow> (c!j-pes-(actk (as!j))\<rightarrow>c!Suc j))" by auto
-                with b1 have c2: "c@[C']\<in>cpts_pes" using cpts_pes_onemore step_def
-                  by (metis (no_types, lifting) b4 cpts_pes_not_empty last_conv_nth)
-                with c1 have c3: "c @ [C'] \<in> cpts_of_pes (paresys_spec pesf) s0 x0" 
-                  using cpts_of_pes_def[of "paresys_spec pesf" s0 x0] C0_ParSys
-                  by (smt cpts_pes_not_empty length_greater_0_conv mem_Collect_eq nth_append) 
-                moreover
-                from c1 have c4: "(c @ [C']) ! (length (c @ [C']) - 2) = C"
-                  by (metis Suc_1 diff_Suc_1 diff_Suc_eq_diff_pred last_conv_nth length_0_conv 
-                      length_append_singleton lessI nat.discI nth_append)
-                moreover
-                have c5: "(c @ [C']) ! (length (c @ [C']) - 1) = C'" by simp
-                moreover
-                from b1 c1 have c50: "\<forall>j. Suc j < length (c @ [C']) \<longrightarrow> 
-                        ((c @ [C'])!j-pes-(actk ((as@[a])!j))\<rightarrow>(c @ [C'])!Suc j)"
-                   by (smt Suc_1 Suc_lessI Suc_less_eq action.simps(1) b3 b4 c4 
-                     diff_Suc_1 diff_Suc_Suc length_append_singleton nth_append nth_append_length) 
-                ultimately have r1: "(gets C, gets C')\<in>Guar\<^sub>f (the (evtrgfs (getx C k)))" 
-                  using b1 b3 b4 c0 c1 act_cptpes_sat_guar_curevt_new2 [rule_format, of pesf "{s0}" UNIV s0 evtrgfs "c@[C']"]
-                     step_def[of a] parsys_sat_rg all_evts_are_basic evt_in_parsys_in_evtrgfs
-                     by (smt One_nat_def Suc_1 append_is_Nil_conv butlast_snoc diff_Suc_1 
-                       diff_Suc_eq_diff_pred diff_Suc_less insertI1 length_butlast 
-                       length_greater_0_conv not_Cons_self2)
-                
-                from c3 c50 have c51: "\<forall>k i. Suc i < length (c @ [C']) \<longrightarrow>
-                          (\<exists>ca. (c @ [C']) ! i -pes-Cmd ca\<sharp>k\<rightarrow> (c @ [C']) ! Suc i) \<longrightarrow>
-                          (\<exists>ef\<in>all_evts pesf. getx ((c @ [C']) ! i) k = fst ef) " 
-                    using all_evts_are_basic cur_evt_in_specevts [of "c@[C']" pesf] by (metis E\<^sub>e_def) 
-                moreover
-                from b1 b3 c0 have c52: "C-pes-Cmd x\<sharp>k\<rightarrow>C'" using step_def by simp
-                ultimately have "(\<exists>ef\<in>all_evts pesf. getx C k = fst ef)"
-                  using c1 c4 c5
-                  proof -
-                    have f1: "\<forall>k n. \<not> Suc n < length (c @ [C']) \<or>
-                        (\<forall>ca. ((c @ [C']) ! n, Cmd ca\<sharp>k, (c @ [C']) ! Suc n) \<notin> pestran) \<or> 
-                        (\<exists>p. p \<in> all_evts pesf \<and> fst p = getx ((c @ [C']) ! n) k)"
-                      by (metis c51)
-                    have f2: "\<forall>ps. c ! length as = (c @ ps) ! length as"
-                      by (metis (no_types) c1 lessI nth_append)
-                    have "c ! length as = C"
-                      by (metis (no_types) append_Nil c1 diff_Suc_1 id_take_nth_drop 
-                          last_length length_Cons take_0 zero_less_Suc)
-                    then show ?thesis
-                      using f2 f1 by (metis c52 c1 c5 diff_Suc_1 length_append_singleton lessI)
-                  qed
-                then obtain ef where c7: "ef\<in>all_evts pesf \<and> getx C k = fst ef" by auto
-                from c0 have "\<not>(\<exists>e k. act_k = EvtEnt e\<sharp>k)"
-                  by (simp add: get_actk_def) 
-                with b3 b4 c0 have c70: "\<exists>x k. act_k = Cmd x\<sharp>k \<and> eventof a = getx C k \<and> dome (gets C) (eventof a) = domain a"
-                  by simp
-                with a1 b3 c0 have c8: "eventof a = getx C k \<and> dome (gets C) (eventof a) = domain a" 
-                  using get_actk_def[of "Cmd x" k]
-                  by (smt (verit) actk.ext_inject get_actk_def)
-                with a1 b3 b6 c7 have "(dome s1 (E\<^sub>e ef)) \<setminus>\<leadsto> u" 
-                  using gets_def E\<^sub>e_def by (metis fst_conv snd_conv) 
-                moreover
-                with p1 b6 b7 c7 r1 have "(gets C, gets C')\<in>Guar\<^sub>e ef" 
-                  using evt_in_parsys_in_evtrgfs Guar\<^sub>f_def E\<^sub>e_def Guar\<^sub>e_def by metis
-                ultimately show ?case using p1 b6 b7 c7 vpeqc_def E\<^sub>e_def c8 a1 by metis
-              next
-                case (EvtEnt x) 
-                from b5 b8 have "s1 = s2" 
-                  using entevt_notchgstate by (metis EvtEnt.prems evtent_is_basicevt)  
-                with b6 b7 show ?case by (simp add: gets_def vpeqc_def vpeq_reflexive)
-              qed
-          }
-          then show ?thesis by auto
-          qed
-      }
-      then show ?thesis using locally_respect_def by simp
-      qed
-    qed
 
 lemma rg_sc_imp_sc: "step_consistent_events \<Longrightarrow> step_consistent"
 proof-
@@ -1378,6 +1264,7 @@ proof-
   qed
 qed
 
+
 theorem UnwindingTheoremE_noninfluence0: 
     assumes p1: observed_consistent
     and     p2: locally_respect_events
@@ -1392,22 +1279,7 @@ theorem UnwindingTheoremE_nonleakage:
   shows nonleakage
   by (simp add: UnwindingTheorem_nonleakage p1 p2 p3 rg_lr_imp_lr rg_sc_imp_sc)
 
-theorem UnwindingTheoremE_noninfluence0_guar:
-    assumes p1: observed_consistent
-    and     p2: locally_respect_events_guar
-    and     p3: step_consistent_events
-  shows     noninfluence0
-  by (simp add: UnwindingTheorem_noninfluence0 p1 p2 p3 rg_lr_guar_imp_lr rg_sc_imp_sc)
-
-theorem UnwindingTheoremE_nonleakage_guar:
-    assumes p1: observed_consistent
-    and     p2: locally_respect_events
-    and     p3: step_consistent_events
-  shows nonleakage
-  by (simp add: UnwindingTheorem_nonleakage p1 p2 p3 rg_lr_imp_lr rg_sc_imp_sc)
 
 end
-
-
 
 end
